examples/delayed_echo/TODOYJ.v
@@ -105,55 +105,6 @@ Definition is_zero (v: val): bool := match v with | Vint x => dec x 0%Z | _ => f
 
 Require Import SimModSem.
 
-Section EXTEND.
-
-  Context `{Σ: GRA.t}.
-
-  Definition extends (stb0 stb1: list (string * fspec)): Prop :=
-    forall fn fnf (FIND: List.find (fun '(_fn, _) => dec fn _fn) stb0 = Some fnf),
-      List.find (fun '(_fn, _) => dec fn _fn) stb1 = Some fnf.
-
-  Global Program Instance extends_PreOrder: PreOrder extends.
-  Next Obligation.
-  Proof.
-    ii. auto.
-  Qed.
-  Next Obligation.
-  Proof.
-    ii. eapply H in FIND. eapply H0 in FIND. auto.
-  Qed.
-
-  Lemma nodup_incl_extends stb0 stb1
-        (INCL: List.incl stb0 stb1)
-        (NODUP: NoDup (List.map fst stb1))
-    :
-      extends stb0 stb1.
-  Proof.
-  Admitted.
-
-  (* Lemma modsempair_extends (md_tgt md_src0 md_src1: ModSemL.t) *)
-  (*         sbtb stb0 stb1 initial_mrs *)
-  (*         (SIM: ModSemLPair.sim (ModSemL.mk (List.map (fun '(fn, fsb) => (fn, fun_to_tgt stb1 fn fsb)) sbtb) initial_mrs) md_tgt) *)
-  (*         (EXTENDS: extends stb0 stb1) *)
-  (*   : *)
-  (*     ModSemLPair.sim (ModSemL.mk (List.map (fun '(fn, fsb) => (fn, fun_to_tgt stb0 fn fsb)) sbtb) initial_mrs) md_tgt. *)
-  (* Proof. *)
-  (*   inv SIM. econs. *)
-  (*   { eapply le_PreOrder. } *)
-  (*   { instantiate (1:=wf). simpl in *. revert sim_fnsems. *)
-  (*     generalize (ModSemL.fnsems md_tgt). induction sbtb. *)
-  (*     { i. inv sim_fnsems. econs. } *)
-  (*     i. destruct a as [fn fb]. inv sim_fnsems. simpl in *. econs. *)
-  (*     2: { eapply IHsbtb. auto. } *)
-  (*     destruct y as [fn' tr]. inv H1. econs. *)
-  (*     { unfold RelationPairs.RelCompFun in *. simpl in *. subst. auto. } *)
-  (*     { unfold RelationPairs.RelCompFun in *. simpl in *. subst. ii. *)
-  (*       exploit H0; [apply H|apply SIMMRS|]. i. des. exists n. *)
-  (*       clear - EXTENDS x0. revert x0. *)
-  (* Admitted. *)
-
-End EXTEND.
-
 
 
 Create HintDb stb.
